verification/tests/DepositTests.dfy
@@ -16,29 +16,28 @@ module DepositTests {
   method PriceDiscoveryTest()
   {
     var cfg := Cfg.DummyConfig().(mechanic := PriceDiscovery);
-    var investment := DummyInvestment();
 
-    var (newInv, newTotalDep, newTotalSold) :=
-      DepositPriceDiscoverySpec(100, 100, 500, 500, investment);
+    var (newAmount, newWeight, newTotalDeposited, newTotalSold) :=
+      DepositPriceDiscoverySpec(100, 100, 500, 500);
 
-    assert newInv.amount == investment.amount + 100;
-    assert newInv.weight == investment.weight + 100;
-    assert newTotalDep == 500 + 100;
+    assert newAmount == 100;
+    assert newWeight == 100;
+    assert newTotalDeposited == 500 + 100;
     assert newTotalSold == 500 + 100;
   }
 
   method FixedPrice_NoRefundTest()
   {
     var cfg := Cfg.DummyConfig().(mechanic := FixedPrice(1, 1));
-    var investment := DummyInvestment();
 
-    var (newInv, newTotalDep, newTotalSold, refund) := 
-    DepositFixedPriceSpec(cfg, 100, 5000, 5000, 150, investment, 1, 1);
+    var (newAmount, newWeight, newTotalDeposited, newTotalSold, newRefund, newAssetsExcess) :=
+      DepositFixedPriceSpec(cfg, 100, 5000, 5000, 150, 1, 1);
 
-    assert refund == 0;
+    assert newRefund == 0;
+    assert newAssetsExcess == 0;
+    assert newAmount == 100;
+    assert newWeight == 100;
+    assert newTotalDeposited == 5000 + 100;
     assert newTotalSold == 5000 + 100;
-    assert newInv.amount == investment.amount + 100;
-    assert newInv.weight == investment.weight + 100;
-    assert newTotalDep == 5000 + 100;
   }
 }
